proof/theories/Red_Ct_Untracked.v
@@ -47,7 +47,7 @@ Import ListNotations.
 Definition e_noentry : env :=
   {| e_set := fun _ => []; e_vmap := fun _ => []; e_map := fun _ => [];
      e_routes := []; e_rt := fun _ => []; e_limit := fun _ => 0;
-     e_quota := fun _ => 0; e_ifaddr := fun _ => []; e_ifaddr6 := fun _ => [];
+     e_quota := fun _ => 0; e_ifaddrs := fun _ => []; e_ifaddrs6 := fun _ => [];
      e_connlimit := fun _ => [];
      e_ct := fun _ k => match k with CKmark => [0;0;0;16] | _ => [] end;
      e_nat := fun _ => None; e_numgen := fun _ => 0 |}.
