proof/theories/Red_NatNoAddrDrop.v
@@ -57,7 +57,7 @@ Definition masq_chain : chain := {| c_policy := Drop; c_rules := [ masq_rule ] |
 Definition env_noaddr : env :=
   {| e_set := fun _ => []; e_vmap := fun _ => []; e_map := fun _ => [];
      e_routes := []; e_rt := fun _ => []; e_limit := fun _ => 0;
-     e_quota := fun _ => 0; e_ifaddr := fun _ => []; e_ifaddr6 := fun _ => [];
+     e_quota := fun _ => 0; e_ifaddrs := fun _ => []; e_ifaddrs6 := fun _ => [];
      e_connlimit := fun _ => []; e_ct := fun _ _ => []; e_nat := fun _ => None;
      e_numgen := fun _ => 0 |}.
 
@@ -65,7 +65,7 @@ Definition env_noaddr : env :=
 Definition env_withaddr : env :=
   {| e_set := fun _ => []; e_vmap := fun _ => []; e_map := fun _ => [];
      e_routes := []; e_rt := fun _ => []; e_limit := fun _ => 0;
-     e_quota := fun _ => 0; e_ifaddr := fun _ => [1;2;3;4]; e_ifaddr6 := fun _ => [];
+     e_quota := fun _ => 0; e_ifaddrs := fun _ => ifaddrs_of [1;2;3;4]; e_ifaddrs6 := fun _ => [];
      e_connlimit := fun _ => []; e_ct := fun _ _ => []; e_nat := fun _ => None;
      e_numgen := fun _ => 0 |}.
 
