proof/theories/Router_NatHook.v
@@ -481,8 +481,8 @@ Definition env_noaddr : env :=
   {| e_set := fun _ => []; e_vmap := fun _ => []; e_map := fun _ => [];
      e_routes := []; e_rt := fun _ => []; e_limit := fun _ => 0;
      e_quota := fun _ => 0;
-     e_ifaddr := fun _ => [];          (* NO usable address on any interface *)
-     e_ifaddr6 := fun _ => []; e_connlimit := fun _ => [];
+     e_ifaddrs := fun _ => [];          (* NO usable address on any interface *)
+     e_ifaddrs6 := fun _ => []; e_connlimit := fun _ => [];
      e_ct := fun _ _ => []; e_nat := fun _ => None; e_numgen := fun _ => 0 |}.
 
 Definition pkt_priv_noaddr : packet :=
