proof/theories/Router_Private.v
@@ -397,7 +397,7 @@ Qed.
 Definition env_lan : env :=
   {| e_set := fun _ => []; e_vmap := e_vmap gen_env; e_map := fun _ => [];
      e_routes := []; e_rt := fun _ => []; e_limit := fun _ => 100;
-     e_quota := fun _ => 0; e_ifaddr := fun _ => []; e_ifaddr6 := fun _ => [];
+     e_quota := fun _ => 0; e_ifaddrs := fun _ => []; e_ifaddrs6 := fun _ => [];
      e_connlimit := fun _ => []; e_ct := fun _ _ => cts_new; e_nat := fun _ => None;
      e_numgen := fun _ => 0 |}.
 
